CL comment fixes and general clean up things.
1. Finished the coordinated close example
2. Fixed type class plumbing
3. Added some comments for the chan record
4. Added an init file so that the package init isn't duplicated
5. Made a class for all the ghost state.

new/proof/github_com/goose_lang/goose/model/channel/chan_ghost_state.v
@@ -10,27 +10,27 @@ Record chan_names :=
     unbuffered_state_tracker_name: gname;
  }.
 
-Class closePropTrackerG Σ := ClosePropTrackerG {
+Class chanGhostStateG Σ  `{ffi_sem: ffi_semantics} `{!ffi_interp ffi}  `{!heapGS Σ}  := ChanGhostStateG {
     sender_main_saved_predG :: savedPredG Σ nat;
     close_prop_auth_setG :: auth_setG Σ gname;
+    exchange_tokG :: ghost_varG Σ (bool * val);
+    chan_ctrG :: inG Σ (authR (optionUR (prodR fracR natR)));
   }.
 
-Definition closePropTrackerΣ: gFunctors :=
-  #[ savedPredΣ nat; auth_setΣ gname ].
+Definition chanGhostStateΣ  `{ffi_sem: ffi_semantics} `{!ffi_interp ffi}   : gFunctors :=
+  #[  savedPredΣ nat; auth_setΣ gname; ghost_varΣ (bool * val); GFunctor (authR (optionUR (prodR fracR natR))) ].
 
-#[global] Instance subG_closePropTrackerG Σ : subG closePropTrackerΣ Σ → closePropTrackerG Σ.
+#[global] Instance subG_chanGhostStateG Σ  `{ffi_sem: ffi_semantics} `{!ffi_interp ffi}  `{!heapGS Σ}  : subG chanGhostStateΣ Σ → chanGhostStateG Σ.
 Proof. solve_inG. Qed.
     
 Set Default Proof Using "Type".
 Set Default Goal Selector "!".
 
 Section lemmas.
-Context `{!ffi_interp ffi}.
-Context `{!inG Σ (authR (optionUR (prodR fracR natR)))}.
-Context `{!closePropTrackerG Σ}.
-Context `{heapGS Σ}.
+Context `{ffi_syntax}.
+Context `{!ffi_model, !ffi_semantics _ _, !ffi_interp _, !heapGS Σ}.
 Implicit Types (v:val).  
-Context `{!ghost_varG Σ (bool * val)}.
+Context  `{!chanGhostStateG Σ}.
 
 Definition own_chan_counter_frag 
 (γ : gname) (n : nat) (q : Qp) : iProp Σ :=
@@ -53,7 +53,6 @@ Definition own_recv_counter_frag (γ: chan_names) (n: nat) (q: Qp) : iProp Σ :=
 Definition own_recv_counter_auth (γ : chan_names) 
   (n : nat) (frozen : bool) : iProp Σ :=
   own_chan_counter_auth γ.(receiver_name) n frozen.
-
 
 Lemma chan_counter_elem (γ: gname) (n: nat) (i: nat) :
  ∀ frozen,
@@ -354,7 +353,6 @@ Lemma own_chan_counter_alloc :
       done.
 Qed.
 
-
 Definition own_close_perm (γ: chan_names) (R:nat -> iProp Σ) (n: nat): iProp Σ :=
   (R n) ∗ own_send_counter_frag γ n 1 ∗ own_closed_tok_auth γ R.
 
@@ -478,7 +476,6 @@ Proof.
   iApply (ghost_var_update (true, #()) with "Htok").
 Qed.
 
-
 Lemma exchange_token_split {T'} `{!IntoVal T'} γ sender_initiated (v: T') :
   full_exchange_token γ ==∗ exchange_token γ sender_initiated v ∗ exchange_token γ sender_initiated v.
 Proof.
@@ -511,7 +508,6 @@ Proof.
   iMod (ghost_var_update (false, #()) with "Htok") as "[Htok1 Htok2]".
   iFrame. done.
 Qed.
-
 
 Lemma sender_exchange_token_combine {T'} `{!IntoVal T'} γ (v v' : T') :
   sender_exchange_token γ v ∗ sender_exchange_token γ v' ==∗ full_exchange_token γ.
