new/proof/github_com/goose_lang/goose/testdata/examples/channel.v
@@ -1,4 +1,3 @@
-
 From New.proof Require Import proof_prelude.
 From New.proof.github_com.goose_lang.goose.model.channel Require Import chan_spec_inv chan_ghost_state chan_spec_api chan_spec_base.
 From New.code.github_com.goose_lang.goose.testdata.examples Require Import channel.
@@ -8,14 +7,182 @@ From Perennial.Helpers Require Import bytes.
 From Coq Require Import Program.Equality.
 Set Default Proof Using "Type*".
 
-
 Section proof.
-    Context `{hG: heapGS Σ, !ffi_semantics _ _}. 
-   Context `{!closePropTrackerG Σ,  !inG Σ (authR (optionUR (prodR fracR natR)))}.
-   Implicit Types (v:val). 
-   Context `{!ghost_varG Σ (bool * val)}.
-   Context `{!goGlobalsGS Σ}.
-   #[global] Program Instance : IsPkgInit chan_spec_raw_examples := ltac2:(build_pkg_init ()).
+Context `{hG: heapGS Σ, !ffi_semantics _ _}. 
+Context  `{!chanGhostStateG Σ}.
+Context `{!ghost_varG Σ (w64)}.
+Context `{!goGlobalsGS Σ}.
+#[global] Program Instance : IsPkgInit chan_spec_raw_examples := ltac2:(build_pkg_init ()).
+
+Lemma wp_CoordinatedChannelClose (γ: chan_names):
+  {{{ is_pkg_init chan_spec_raw_examples }}}
+    chan_spec_raw_examples @ "CoordinatedChannelClose" #()
+  {{{ RET #(); True }}}.
+Proof.
+  wp_start; wp_auto.
+  wp_apply wp_fupd.
+
+  (* Allocate two ghost variables for distinguishing send cases *)
+  iMod (ghost_var_alloc (W64 42)) as (γs1) "HSend42".
+  iMod (ghost_var_alloc (W64 84)) as (γs2) "HSend84".
+
+  (* Allocate buffered channel for sending 42 or 84 *)
+  wp_apply (wp_NewChannelRef_base w64
+    2 (* buffered size *)
+    false (* single party *)
+    (λ i (v: w64), emp)%I
+    (λ (v:w64),
+      (ghost_var γs1 1%Qp (W64 42) ∗ ⌜v = W64 42⌝) ∨
+      (ghost_var γs2 1%Qp (W64 84) ∗ ⌜v = W64 84⌝)
+    )%I
+    (λ i, True)%I
+    True%I
+    (λ n, ⌜n = 2%nat⌝)%I).
+  all: try done.
+  iIntros (buf_ch mu1 ch_buf_slice1 γ1 buff_params) "Hbuffchan".
+  iNamed "Hbuffchan". iDestruct "HCh" as "#HCh".
+  iDestruct "Hbuffchan" as "[Hclosedtok Hrest]". iNamed "Hrest".
+  iModIntro.
+  wp_auto.
+
+  (* Allocate unbuffered sync channel for controlling coordination *)
+  wp_apply (wp_NewChannelRef_base w64
+    0 (* unbuffered *)
+    true (* single party *)
+    (λ i _, if decide (i = 0) then own_send_counter_frag (buff_params.(ch_γ w64)) 1 (1/2)%Qp else False)%I
+    (λ (v: w64), True)%I
+    (λ i, True)%I
+    True%I
+    (λ n, False)%I).
+  all: try done.
+  iIntros (sync_ch mu2 ch_buf_slice2 γ2 sync_params) "(%Hsyncparams & #Hsyncchan & Hctsync & HScsync & HRecvPermSync)".
+  wp_auto.
+  iNamed "HCh".
+  iDestruct "Hsyncchan" as "(#musync  & #buffsync & %Hbuffsizesync & %Hbuffltsync & %Hmaxsync & #Hlocksync)".
+
+  (* Ensure channels are valid (non-null) *)
+  iDestruct (chan_pointsto_non_null w64 (buff_params.(ch_mu w64)) buff_params with "mu") as %HBufNonNull.
+  assert (buff_params.(ch_loc w64) ≠ null) as HBufNotNull by (intro; congruence).
+  iDestruct (chan_pointsto_non_null w64 (sync_params.(ch_mu w64)) sync_params with "musync") as %HSyncNonNull.
+  assert (sync_params.(ch_loc w64) ≠ null) as HSyncNotNull by (intro; congruence).
+  iPersist "syncCh" as "#syncCh".
+  iPersist "bufCh" as "#bufCh".
+  iDestruct "HSc" as "[HMainBuffSend HForkBuffSend]".
+  iDestruct "Hparams" as "%".
+
+  (* Fork worker thread to send 42 and 0 *)
+  wp_apply (wp_fork with "[HScsync HForkBuffSend HSend42]").
+  {
+
+    replace sync_ch with (sync_params.(ch_loc w64)) by (subst;done).
+    replace buf_ch with buff_params.(ch_loc w64) by (subst;done).
+    (* Send 42 on buffered channel *)
+    wp_apply ((wp_Channel__Send w64 buff_params 0%nat (1/2)%Qp (W64 42)) with "[HForkBuffSend HSend42 bufCh]"). all: try (subst;done).
+    { 
+      iFrame "#%". unfold P. iFrame. subst. simpl. iSplitL "";first done. 
+      iLeft. iFrame. done.
+    }
+    iIntros "HSendDone".
+    wp_auto.
+
+    (* Send 0 on sync channel to join forked sender so we can safely close *)
+    wp_apply ((wp_Channel__Send w64 sync_params 0%nat 1%Qp (W64 0)) with "[HScsync syncCh HSendDone]").
+    all: try (subst;done).
+    { iFrame "#". subst. simpl. unfold send_post. simpl. iDestruct "HSendDone" as "[_ Hsc]".
+      iFrame. iPureIntro; done. }
+    iIntros "_".
+    wp_auto. done.
+  }
+
+  replace sync_ch with (sync_params.(ch_loc w64)) by (subst;done).
+  replace buf_ch with buff_params.(ch_loc w64) by (subst;done).
+  (* Send 84 on buffered channel *)
+  wp_apply ((wp_Channel__Send w64 buff_params 0%nat (1/2)%Qp (W64 84)) with "[bufCh HMainBuffSend HSend84]"). all: try (subst;done).
+  { iFrame "#". unfold P. subst. simpl. iFrame "%". iFrame. iSplitL "";first done.
+    iRight. iFrame. done. 
+  }
+  iIntros "HSendDone84".
+  wp_auto.
+
+  (* Receive discard from sync channel *)
+  wp_apply ((wp_Channel__ReceiveDiscardOk w64 sync_params 0%nat 1%Qp (λ n, False)%I) with "[HRecvPermSync]").
+  {
+    subst. simpl. iFrame "%".
+    iFrame. iFrame "#". iPureIntro; done.
+  }
+  iIntros (v ok) "HRecvSync".
+  wp_auto.
+  iDestruct "HSendDone84" as "[_ Hscf]".
+
+  destruct ok.
+  - (* Proceed to close the buffered channel *)
+    unfold recv_post.
+    iDestruct "HRecvSync" as "[HMainBufSend HRcp]".
+    wp_apply ((wp_Channel__Close w64 buff_params 2) with "[HMainBufSend Hscf Hclosedtok]").
+    all: try (subst;done).
+    { subst. simpl. iFrame. iFrame "#". iFrame "%". unfold send_post. 
+      (* Put the send permissions back together *)
+      iCombine "HMainBufSend Hscf" as "Hcperm".
+      iFrame. iPureIntro;done.
+    }
+
+    (* Receive both values from buffered channel *)
+    wp_apply ((wp_Channel__Receive w64 buff_params 0%nat 1%Qp (λ n, ⌜n = 2%nat⌝)%I) with "[HRecvPerm]").
+    { subst. simpl. iFrame. iFrame "#". iFrame "%". iPureIntro; done. }
+    iIntros (v0 ok0) "HRecv1".
+    wp_auto.
+
+    destruct ok0.
+    + iDestruct "HRecv1" as "[HP Hrecvperm]". unfold P.
+      wp_apply ((wp_Channel__Receive w64 buff_params 1%nat 1%Qp (λ n, ⌜n = 2%nat⌝)%I) with "[Hrecvperm]").
+        { 
+          subst. simpl. iFrame. iFrame "#". iFrame "%". simpl. iPureIntro; done. 
+        }
+        iIntros (v1 ok1) "HRecv2".
+        wp_auto.
+
+        destruct ok1.
+      *
+
+       unfold recv_post.
+      iDestruct "HRecv2" as "[HP2 HRecvPerm2]". unfold P. subst. simpl.
+      (* Handle possible orderings of buffered results *)
+       iDestruct "HP" as "[[Hg42 %H42]|[Hg84 %H84]]". 
+       {
+        iDestruct "HP2" as "[[Hg42' %H42']|[Hg84' %H84']]".  
+        {
+          subst v1. simpl. subst v0.   
+          iCombine "Hg42 Hg42'" as "Hinvalid" gives "(%Hinvalid & %Hv)".
+          done.  
+        }
+        {
+         subst v1. simpl. subst v0. wp_auto. iApply "HΦ". done. 
+        }
+       }
+       {
+        iDestruct "HP2" as "[[Hg42' %H42']|[Hg84' %H84']]".  
+        {
+         subst v1. simpl. subst v0. wp_auto. iApply "HΦ". done. 
+        }
+        {
+          subst v1. simpl. subst v0.   
+          iCombine "Hg84 Hg84'" as "Hinvalid" gives "(%Hinvalid & %Hv)".
+          done.  
+        }
+       }
+      * wp_auto. iNamed "HRecv2". iNamed "HRecv2". unfold own_recv_perm.
+        iNamed "HRcp". iDestruct "HRi" as "%". 
+        iDestruct "HRcp" as "[HRcp Hoct]".
+        subst n.
+        (* We must receive 2 elements which we contracted through Ri, can't be closed here *)
+        iDestruct (recv_counter_elem buff_params.(ch_γ w64)  with "[$Hrca] [$HRecFrag]") as "%Hag2".
+        done.
+    + iNamed "HRecv1". iNamed "HRecv1". iDestruct "HRi" as "%". subst n.
+      iDestruct (recv_counter_elem buff_params.(ch_γ w64)  with "[$Hrca] [$HRecFrag]") as "%Hag2".
+      done.
+  - (* We agreed not to close the sync channel in sync_params R *)
+    iNamed "HRecvSync". iNamed "HRecvSync". done. 
+Qed.
 
 Definition hello_world_pred
 (z: Z) (v: byte_string): iProp Σ :=
@@ -23,73 +190,57 @@ Definition hello_world_pred
 .
 
 Lemma wp_SendMessage (γ: chan_names):
-   {{{ is_pkg_init chan_spec_raw_examples }}}
-     chan_spec_raw_examples @ "SendMessage" #()
-   {{{ RET #();
-       True
-   }}}.
- Proof.
-  wp_start; wp_auto. 
-  set par := make_unbuffered_params_simple_single_sync byte_string stringT _ _ _ messageChan_ptr γ hello_world_pred. 
-  unfold make_unbuffered_params_simple_single_sync in par.
-  replace 0 with par.(ch_size) by trivial.
-  wp_apply ((wp_NewChannelRef par) with "[]").
-  iIntros (ch_ref_ptr). iIntros "Hch". iNamed "Hch". iNamed "HCh".
+  {{{ is_pkg_init chan_spec_raw_examples }}}
+    chan_spec_raw_examples @ "SendMessage" #()
+  {{{ RET #(); True }}}.
+Proof.
+  wp_start; wp_auto.
+
+  (* Allocate an unbuffered sync channel with hello_world_pred *)
+  wp_apply (wp_NewChannelRef_simple_unbuffered_sync
+              byte_string
+              hello_world_pred).
+  iIntros (msg_ch_ptr mu ch_buf_slice ch_γ_names params) "HChan".
+  iNamed "HChan". iNamed "HCh".
   wp_auto.
-  iDestruct ((chan_pointsto_non_null mu_l par) with "[Hlock]") as %Hnotnull;trivial.
-     assert (par.(ch_loc) ≠ null).
-    {
-      intro H.
-      replace (par.(ch_loc)) with null in Hnotnull.
-      done.
-    }
+
+  (* Validate channel pointer is non-null *)
+  iDestruct (chan_pointsto_non_null byte_string (params.(ch_mu byte_string)) params with "mu") as %HMsgNonNull.
+  assert (params.(ch_loc byte_string) ≠ null) as HMsgNotNull by (intro; congruence).
   iPersist "messageChan" as "#messageChan".
+
+  (* Fork off sender thread *)
   wp_apply (wp_fork with "[HSc]").
   {
-    replace stringT with (par.(ch_T)) by trivial.
-    replace ch_ref_ptr with (par.(ch_loc)) by trivial.
-    wp_apply (( wp_Channel__Send par 0%nat "hello world"%go) with "[HSc]").
-    {
-      done.
-    }
-    {
-      trivial.
-    }
-    {
-     iFrame. iFrame "#". unfold P. iPureIntro.
-    done.
-    }
-    {
-     iIntros "H". wp_auto. done. 
-    }
+    replace msg_ch_ptr with (params.(ch_loc byte_string)) by (subst;done).
+    (* Send "hello world" on the message channel *)
+    wp_apply ((wp_Channel__Send byte_string params 0%nat 1%Qp "hello world"%go) with "[messageChan HSc]").
+    all: try (subst;done).
+    { iFrame "#". iFrame "%". iFrame. unfold P. subst. simpl. iFrame. iPureIntro; done. }
+    iIntros "_". wp_auto. done.
   }
-    replace stringT with (par.(ch_T)) by trivial.
-    replace ch_ref_ptr with (par.(ch_loc)) by trivial.
-    wp_apply (( wp_Channel__ReceiveDiscardOk par 0%nat) with "[HRecvPerm]").
-    {
-      done.
-    }
-    {
-     iFrame. iFrame "#". iPureIntro. split.
-     {
-      done.
-     }
-     done. 
-    }
-    iIntros (v). iIntros (ok). iIntros "HRecPost". unfold recv_post.
-     wp_auto. 
-     destruct ok.
-     {
-      unfold P. simpl. iDestruct "HRecPost" as "[%Hhwpred Hrecvperm]".
-      subst v. destruct bool_decide eqn: Hobv.
-      {
-        wp_auto. iApply "HΦ". done.
-      }
-      done.
-     }
-     iNamed "HRecPost".
-     iNamed "HRecPost".
-     done.
- Qed.
+
+  replace msg_ch_ptr with (params.(ch_loc byte_string)) by (subst;done).
+  (* Main thread discards the received message *)
+  wp_apply ((wp_Channel__ReceiveDiscardOk byte_string params 0%nat) with "[HRecvPerm]").
+  {
+    iFrame "#".
+    unfold Q. subst. simpl. iFrame. iPureIntro; done.
+  }
+  iIntros (v ok) "HRecvPost".
+  wp_auto.
+
+  destruct ok.
+  - (* Received successfully *)
+    unfold recv_post, hello_world_pred.
+    iDestruct "HRecvPost" as "[HP HRecvPerm]".
+    unfold P. subst. simpl. iDestruct "HP" as "%HP".
+    subst v.
+    destruct bool_decide eqn:HDecide.
+    + wp_auto. iApply "HΦ". done.
+    + done.
+  - (* We agreed not to close *)
+    iNamed "HRecvPost". iNamed "HRecvPost". done.
+Qed.
 
 End proof.
